theories/Commons/Language.v
@@ -3,18 +3,18 @@ From RSL Require Import Prelude.
 From RSL.Commons Require Export Memory Values.
 
 Section lang_mixin.
-  Context {prog istate value : Type}.
+  Context {prog state value : Type}.
 
-  Context (step_rel : prog -> (istate * memory) -> (istate * memory) -> Prop).
-  Context (is_value : istate -> option value).
+  Context (step_rel : prog -> (state * memory) -> (state * memory) -> Prop).
+  Context (is_value : state -> option value).
 
   Record LangMixin := {
       mixin_final_no_step s v:
         is_value s = Some v -> ∀ m p s', ~step_rel p (s, m) s';
 
-      mixin_can_step_mono p s m t mm:
-        step_rel p (s, m) t ->
-        (∃ t', step_rel p (s, m ∪ mm) t')
+      mixin_step_mono p s m c mm:
+        step_rel p (s, m) c ->
+        (∃ c', step_rel p (s, m ∪ mm) c')
     }.
 End lang_mixin.
 
@@ -22,11 +22,11 @@ Structure lang :=
   Lang
     {
       prog : Type;
-      istate : Type;
+      state : Type;
       value : Type;
 
-      step_rel : prog -> (istate * memory) -> (istate * memory) -> Prop;
-      is_value : istate -> option value;
+      step_rel : prog -> (state * memory) -> (state * memory) -> Prop;
+      is_value : state -> option value;
 
       lang_mixin : LangMixin step_rel is_value;
     }.
@@ -39,9 +39,9 @@ Notation "P ⊨ s '-{' n '}>' t" := (nsteps (step_rel P) n s t) (at level 60, ri
 Notation "P ⊨ s '->>*' t" := (rtc (step_rel P) s t) (at level 60, right associativity).
 Notation "P ⊨ s '->>+' t" := (psteps (step_rel P) s t) (at level 60, right associativity).
 
-Definition state (Λ: lang) : Type := istate Λ * memory.
+Definition config (Λ: lang) : Type := state Λ * memory.
 
-Definition is_final {Λ : lang} (s: state Λ) :=
+Definition is_final {Λ : lang} (s: config Λ) :=
   let '(ps, m) := s in
   match is_value ps with
   | Some v => Some (v, m)
@@ -50,53 +50,49 @@ Definition is_final {Λ : lang} (s: state Λ) :=
 
 Section LangProp.
   Context {Λ: lang} (P: prog Λ).
-  Implicit Types (s : state Λ) (v : value Λ) (ss: istate Λ).
+  Implicit Types (c : config Λ) (v : value Λ) (s: state Λ).
 
-  Lemma is_final_Some s v m:
-    is_final s = Some (v, m)
-    <->
-      ∃ ps, s = (ps, m) ∧ is_value ps = Some v.
+  Lemma is_final_Some c v m:
+    is_final c = Some (v, m) <-> ∃ s, c = (s, m) ∧ is_value s = Some v.
   Proof using Type.
     split.
-    - destruct s as [ps ?]. simpl.
-      destruct (is_value ps) eqn:Hp; intros H; inv H.
+    - destruct c as [s ?]. simpl.
+      destruct (is_value s) eqn:Hp; intros H; inv H.
       eexists. by split.
-    - intros (ps & -> & Hfin). simpl. by rewrite Hfin.
+    - intros (s & -> & Hfin). simpl. by rewrite Hfin.
   Qed.
 
-  Local Lemma is_final_None s:
-    is_final s = None
-    <->
-      ∃ ps m, s = (ps, m) ∧ is_value ps = None.
+  Local Lemma is_final_None c:
+    is_final c = None <-> ∃ s m, c = (s, m) ∧ is_value s = None.
   Proof using Type.
     split.
-    - destruct s as [ps m]. simpl.
-      destruct (is_value ps) eqn:Hp; intros H; inv H.
-      eexists ps, m. by split.
-    - intros (ps & m & -> & Hfin). simpl. by rewrite Hfin.
+    - destruct c as [s m]. simpl.
+      destruct (is_value s) eqn:Hp; intros H; inv H.
+      eexists s, m. by split.
+    - intros (s & m & -> & Hfin). simpl. by rewrite Hfin.
   Qed.
 
-  Lemma final_no_step s:
-    is_Some (is_final s) -> ∀ t, ~(P ⊨ s ->> t).
+  Lemma final_no_step c:
+    is_Some (is_final c) -> ∀ c', ~(P ⊨ c ->> c').
   Proof using Type.
-    intros [[] (ps & -> & Hfin)%is_final_Some] t.
+    intros [[] (s & -> & Hfin)%is_final_Some] t.
     eapply mixin_final_no_step.
     - apply lang_mixin.
     - exact Hfin.
   Qed.
 
-  Definition can_progress s: Prop := ∃ t, P ⊨ s ->> t.
+  Definition can_progress c: Prop := ∃ c', P ⊨ c ->> c'.
 
-  Definition stuck s : Prop := is_final s = None ∧ ~ can_progress s.
+  Definition stuck c : Prop := is_final c = None ∧ ~ can_progress c.
 
-  Lemma can_progress_must_step s:
-    can_progress s -> ∃ t, P ⊨ s ->> t.
+  Lemma can_progress_must_step c:
+    can_progress c -> ∃ c', P ⊨ c ->> c'.
   Proof using Type. easy. Qed.
 
-  Lemma final_no_progress s:
-    is_Some (is_final s) -> ~can_progress s.
+  Lemma final_no_progress c:
+    is_Some (is_final c) -> ~can_progress c.
   Proof using Type.
-    intros [[] (ps & -> & Hfin)%is_final_Some] Hp.
+    intros [[] (s & -> & Hfin)%is_final_Some] Hp.
     destruct (can_progress_must_step _ Hp) as (? & H).
     eapply mixin_final_no_step.
     - apply lang_mixin.
@@ -104,52 +100,52 @@ Section LangProp.
     - exact H.
   Qed.
 
-  Lemma final_not_stuck s:
-    is_Some (is_final s) -> ~ stuck s.
+  Lemma final_not_stuck c:
+    is_Some (is_final c) -> ~ stuck c.
   Proof using Type.
     intros [[] Hfin] [Hnstuck _]. congruence.
   Qed.
 
-  Lemma progress_not_stuck s:
-    can_progress s -> ~ stuck s.
+  Lemma progress_not_stuck c:
+    can_progress c -> ~ stuck c.
   Proof using Type. intros H [_ Hnprog]. by eapply Hnprog. Qed.
 
-  Lemma progress_not_final s:
-    can_progress s -> is_final s = None.
+  Lemma progress_not_final c:
+    can_progress c -> is_final c = None.
   Proof using Type.
-    intros (s' & ?)%can_progress_must_step.
-    destruct (is_final s) eqn:Hfin; auto.
+    intros (c' & ?)%can_progress_must_step.
+    destruct (is_final c) eqn:Hfin; auto.
     exfalso.
     by eapply final_no_step.
   Qed.
 
-  Lemma is_final_mem_ignore ss m m1 m2 v :
-    is_final (ss, m1) = Some (v, m) ->
-    is_final (ss, m2) = Some (v, m2).
+  Lemma is_final_mem_ignore s m m1 m2 v :
+    is_final (s, m1) = Some (v, m) ->
+    is_final (s, m2) = Some (v, m2).
   Proof using Type.
     intros (? & He & Hfin)%is_final_Some.
     inv He. simpl. by rewrite Hfin.
   Qed.
 
-  Lemma is_final_mem_same ss m m' v :
-    is_final (ss, m) = Some (v, m') ->
+  Lemma is_final_mem_same s m m' v :
+    is_final (s, m) = Some (v, m') ->
     m = m'.
   Proof using Type.
     intros (? & He & Hfin)%is_final_Some. by inv He.
   Qed.
 
-  Lemma can_progress_mono ss m mm:
-    can_progress (ss, m) ->
-    can_progress (ss, m ∪ mm).
+  Lemma can_progress_mono s m mm:
+    can_progress (s, m) ->
+    can_progress (s, m ∪ mm).
   Proof using Type.
     intros (t & Hstep).
-    eapply (mixin_can_step_mono _ _ (lang_mixin Λ)) in Hstep as (t' & Hstep).
+    eapply (mixin_step_mono _ _ (lang_mixin Λ)) in Hstep as (t' & Hstep).
     by eexists.
   Qed.
 
-  Lemma stuck_anti_mono ss m mm:
-    stuck (ss, m ∪ mm) ->
-    stuck (ss, m).
+  Lemma stuck_anti_mono s m mm:
+    stuck (s, m ∪ mm) ->
+    stuck (s, m).
   Proof using Type.
     intros [(? & ? & Heq & Hval)%is_final_None Hnprog].
     split.
@@ -157,13 +153,14 @@ Section LangProp.
     - intro Hp. apply Hnprog, can_progress_mono, Hp.
   Qed.
 
-  Definition super_stuck '(ss, m) :=
-    is_value ss = None ∧ ∀ mm, ~can_progress (ss, m ∪ mm).
+  Definition super_stuck (c: config Λ) : Prop :=
+    let '(s, m) := c in
+    is_value s = None ∧ ∀ mm, ~can_progress (s, m ∪ mm).
 
-  Lemma super_stuck_is_stuck s :
-    super_stuck s -> stuck s.
+  Lemma super_stuck_is_stuck c:
+    super_stuck c -> stuck c.
   Proof using Type.
-    destruct s as [ss m].
+    destruct c as [s m].
     intros [Hval Hnprog].
     split.
     - apply is_final_None. by eexists _, _.
@@ -171,9 +168,9 @@ Section LangProp.
       unfold memory. by rewrite map_union_empty.
   Qed.
 
-  Lemma super_stuck_mono ss m mm:
-    super_stuck (ss, m) ->
-    super_stuck (ss, m ∪ mm).
+  Lemma super_stuck_mono s m mm:
+    super_stuck (s, m) ->
+    super_stuck (s, m ∪ mm).
   Proof using Type.
     intros [Hval Hnprog].
     split; first done.
@@ -188,7 +185,7 @@ Section TwoProg.
   Context {Λt Λs: lang}.
   Context (Pt : prog Λt) (Ps : prog Λs).
 
-  Definition both_final ϕ (t: state Λt) (s: state Λs) : Prop :=
+  Definition both_final ϕ (t: config Λt) (s: config Λs) : Prop :=
     ∃ vt vs mt ms,
       is_final t = Some (vt, mt) ∧
       is_final s = Some (vs, ms) ∧
